cedar-lean/Cedar/Thm/BatchedEvaluator/Evaluate.lean
@@ -26,27 +26,28 @@ theorem batched_evaluate_loop_eq_evaluate
   (es : Entities)
   {current_store : PartialEntities}
   {env : TypeEnv} :
-  EntityLoader.WellBehaved es loader →
+  req.context.WellFormed →
+  EntityLoader.WellBehaved env.ets es loader →
   Residual.WellTyped env x →
-  RequestAndEntitiesRefine req es req.asPartialRequest current_store →
+  RequestAndEntitiesRefine req es (req.asPartialRequest env.reqty.context) current_store →
   InstanceOfWellFormedEnvironment req es env →
   (Residual.evaluate (batchedEvaluateLoop env x req loader current_store iters) req es).toOption = (Residual.evaluate x req es).toOption := by
-  intro h₀ h₁ h₂ h₃
+  intro hctxwf h₀ h₁ h₂ h₃
   unfold batchedEvaluateLoop
   split
   case h_1 => simp only
   case h_2 iters n=>
     let toLoad := (Set.filter (fun uid => (Map.find? current_store uid).isNone) x.allLiteralUIDs)
-    let newEntities := ((loader toLoad).mapOnValues MaybeEntityData.asPartial)
+    let newEntities := SlicedEntities.asPartial env.ets (loader toLoad)
     let newStore := newEntities ++ current_store
 
-    have h₆ : RequestAndEntitiesRefine req es req.asPartialRequest newStore := by
+    have h₆ : RequestAndEntitiesRefine req es (req.asPartialRequest env.reqty.context) newStore := by
       constructor
-      · exact as_partial_request_refines
+      · exact as_partial_request_refines hctxwf
       · apply entities_refine_append
         · exact h₂.right
-        · exact (h₀ toLoad).2
-    let newRes := TPE.evaluate env x req.asPartialRequest newStore
+        · exact (h₀ toLoad)
+    let newRes := TPE.evaluate env x (req.asPartialRequest env.reqty.context) newStore
     have h₇ : (Residual.evaluate newRes req es).toOption = (Residual.evaluate x req es).toOption := by
       rw [← partial_evaluate_is_sound h₁ h₃ h₆]
 
@@ -57,7 +58,7 @@ theorem batched_evaluate_loop_eq_evaluate
       exact h₇
     case h_2 =>
       have h₈ := (partial_eval_preserves_well_typed h₃ h₆ h₁)
-      rw [batched_evaluate_loop_eq_evaluate es h₀ h₈ h₆ h₃]
+      rw [batched_evaluate_loop_eq_evaluate es hctxwf h₀ h₈ h₆ h₃]
       exact h₇
 
 
